%%%%%%%%%%%%%%%%%%%%%%%%%%%%%%%%%%%%%%%%%%%%%%%%%%%%%%%%%%%%%%%%%%%%%%
%%%%%%%%%%%%%%%%%%%%%%%%%%%%%%%%%%%%%%%%%%%%%%%%%%%%%%%%%%%%%%%%%%%%%%
%%%%%%%%%%%%%%%%%%%%%%%%%%%%%%%%%%%%%%%%%%%%%%%%%%%%%%%%%%%%%%%%%%%%%%
\newpage
\section{Equivalence-principle PFT (EPPFT)}

In the EPPFT approach, we compute the power, force and torque
on a body $\mc B$ by considering the work done on, and the force and
torque exerted on, the equivalent surface currents $\vb K, \vb N$
flowing on the body surface $\partial \mc B$.

The power may be computed as the Joule heating of the
$\vb K$ and $\vb N$ currents by the $\vb E$ and $\vb H$ fields:
%====================================================================%
\begin{subequations}
\begin{equation}
 P\sups{abs} 
     = \frac{1}{2}\text{ Re }
      \int_{\partial \mc B} \Big[ \vb K^*(\vb x) \cdot \vb E(\vb x)
                                 +\vb N^*(\vb x) \cdot \vb H(\vb x)
                            \Big] \, dA
\end{equation}
\end{subequations}
%====================================================================%

Assuming we are in a lossless region so $k$ is real-valued, one finds
%====================================================================%
\begin{align*}
P\sups{abs}
&=\frac{k}{2}\text{Re }\sum_{\alpha\beta}
  \left[ k_\alpha^*
         \bigg( iZ_0G_{\alpha\beta} k_\beta + iC_{\alpha\beta}n_\beta \bigg)
        +n_\alpha^*
         \left( -iC_{\alpha\beta} k_\beta + 
                \frac{i}{Z_0}G_{\alpha\beta}n_\beta \right)
 \right]
\intertext{Write out the $\text{Re}$ operation:}
&=\frac{k}{4}\sum_{\alpha\beta}\bigg\{
  \left[ k_\alpha^*
         \bigg( iZ_0G_{\alpha\beta} k_\beta + iC_{\alpha\beta}n_\beta \bigg)
        +n_\alpha^*
         \left( -iC_{\alpha\beta} k_\beta + 
                \frac{i}{Z_0}G_{\alpha\beta}n_\beta \right)
  \right] \\
&\quad\qquad\,\,\,\, + 
  \left[ k_\alpha
         \bigg(-iZ_0G^*_{\alpha\beta} k^*_\beta - iC^*_{\alpha\beta}n^*_\beta \bigg)
        +n_\alpha
         \left( +iC^*_{\alpha\beta} k^*_\beta - 
                \frac{i}{Z_0}G^*_{\alpha\beta}n^*_\beta \right)
  \right]\bigg\}
\intertext{Relabel $\alpha \leftrightarrow \beta$ in the second term and
           use $G_{\alpha\beta}=G_{\beta\alpha}$, 
               $C_{\alpha\beta}=-C_{\beta\alpha}$:} 
%====================================================================%
&=\frac{k}{4}\sum_{\alpha\beta}\bigg\{
  \left[ k_\alpha^*
         \bigg( iZ_0G_{\alpha\beta} k_\beta + iC_{\alpha\beta}n_\beta \bigg)
        +n_\alpha^*
         \left( -iC_{\alpha\beta} k_\beta + 
                \frac{i}{Z_0}G_{\alpha\beta}n_\beta \right)
  \right] \\
&\quad\qquad\,\,\,\, + 
  \left[ k^*_\alpha
         \bigg(-iZ_0G^*_{\alpha\beta} k_\beta - iC^*_{\alpha\beta}n_\beta \bigg)
        +n^*_\alpha
         \left( -iC^*_{\alpha\beta} k_\beta - 
                \frac{i}{Z_0}G^*_{\alpha\beta}n_\beta \right)
  \right]\bigg\}
\\
\end{align*}
%====================================================================%
